Verified/IMP/SmallStep.lean
@@ -1,3 +1,4 @@
+import Std
 import Verified.IMP.Syntax
 
 namespace IMP
@@ -8,44 +9,52 @@ namespace IMP
 
 instance : Coe Value Expr := ⟨Value.toExpr⟩
 
-inductive Reduce : Env × Expr -> Env × Expr -> Prop where
-  | var : env x = some v -> Reduce (env, .var x) (env, v)
+inductive Expr.Step : Env × Expr -> Env × Expr -> Prop where
+  | var (h : x ∈ env) :
+    Expr.Step (env, .var x) (env, (env.get x h : Value))
   | add_left :
-    Reduce (env, e1) (env, e1') ->
-    Reduce (env, .add e1 e2) (env, .add e1' e2)
+    Expr.Step (env, e1) (env, e1') ->
+    Expr.Step (env, .add e1 e2) (env, .add e1' e2)
   | add_right :
-    Reduce (env, e2) (env, e2') ->
-    Reduce (env, .add (.num n1) e2) (env, .add (.num n1) e2')
-  | add_val : Reduce (env, .add (.num n1) (.num n2)) (env, .num (n1 + n2))
+    Expr.Step (env, e2) (env, e2') ->
+    Expr.Step (env, .add (.num n1) e2) (env, .add (.num n1) e2')
+  | add_val :
+    Expr.Step (env, .add (.num n1) (.num n2)) (env, .num (n1 + n2))
   | mul_left :
-    Reduce (env, e1) (env, e1') ->
-    Reduce (env, .mul e1 e2) (env, .mul e1' e2)
+    Expr.Step (env, e1) (env, e1') ->
+    Expr.Step (env, .mul e1 e2) (env, .mul e1' e2)
   | mul_right :
-    Reduce (env, e2) (env, e2') ->
-    Reduce (env, .mul (.num n1) e2) (env, .mul (.num n1) e2')
-  | mul_val : Reduce (env, .mul (.num n1) (.num n2)) (env, .num (n1 * n2))
+    Expr.Step (env, e2) (env, e2') ->
+    Expr.Step (env, .mul (.num n1) e2) (env, .mul (.num n1) e2')
+  | mul_val :
+    Expr.Step (env, .mul (.num n1) (.num n2)) (env, .num (n1 * n2))
   | lt_left :
-    Reduce (env, e1) (env, e1') ->
-    Reduce (env, .lt e1 e2) (env, .lt e1' e2)
+    Expr.Step (env, e1) (env, e1') ->
+    Expr.Step (env, .lt e1 e2) (env, .lt e1' e2)
   | lt_right :
-    Reduce (env, e2) (env, e2') ->
-    Reduce (env, .lt (.num n1) e2) (env, .lt (.num n1) e2')
-  | lt_val : Reduce (env, .lt (.num n1) (.num n2)) (env, .bool (n1 < n2))
+    Expr.Step (env, e2) (env, e2') ->
+    Expr.Step (env, .lt (.num n1) e2) (env, .lt (.num n1) e2')
+  | lt_val :
+    Expr.Step (env, .lt (.num n1) (.num n2)) (env, .bool (n1 < n2))
 
-inductive Step : Env × Stmt -> Env × Stmt -> Prop where
-  | assign_reduce :
-    Reduce (env, e) (env, e') ->
-    Step (env, .assign x e) (env, .assign x e')
-  | assign_val (v : Value) : Step (env, .assign x v) (Env.update env x v, .skip)
+inductive Stmt.Step : Env × Stmt -> Env × Stmt -> Prop where
+  | assign_step :
+    Expr.Step (env, e) (env, e') ->
+    Stmt.Step (env, .assign x e) (env, .assign x e')
+  | assign_val (v : Value) :
+    Stmt.Step (env, .assign x v) (env.insert x v, .skip)
   | seq_left :
-    Step (env, s1) (env', s1') ->
-    Step (env, .seq s1 s2) (env', .seq s1' s2)
-  | seq_skip : Step (env, .seq .skip s2) (env, s2)
-  | ite_reduce :
-    Reduce (env, e) (env, e') ->
-    Step (env, .ite e s1 s2) (env, .ite e' s1 s2)
-  | ite_true : Step (env, .ite (.bool true) s1 s2) (env, s1)
-  | ite_false : Step (env, .ite (.bool false) s1 s2) (env, s2)
-  | while : Step (env, .while e s) (env, .ite e (.seq s (.while e s)) .skip)
+    Stmt.Step (env, s1) (env', s1') ->
+    Stmt.Step (env, .seq s1 s2) (env', .seq s1' s2)
+  | seq_skip : Stmt.Step (env, .seq .skip s2) (env, s2)
+  | ite_step :
+    Expr.Step (env, e) (env, e') ->
+    Stmt.Step (env, .ite e s1 s2) (env, .ite e' s1 s2)
+  | ite_true :
+    Stmt.Step (env, .ite (.bool true) s1 s2) (env, s1)
+  | ite_false :
+    Stmt.Step (env, .ite (.bool false) s1 s2) (env, s2)
+  | while :
+    Stmt.Step (env, .while e s) (env, .ite e (.seq s (.while e s)) .skip)
 
 end IMP
