Verified/VAE/SmallStep.lean
@@ -2,41 +2,34 @@ import Verified.VAE.Syntax
 
 namespace VAE
 
-inductive Reduce : Env × Expr -> Env × Expr -> Prop where
+inductive Step : Env × Expr -> Env × Expr -> Prop where
   | add_left :
-    Reduce (env, e1) (env', e1') ->
-    Reduce (env, .add e1 e2) (env', .add e1' e2)
+    Step (env, e1) (env', e1') ->
+    Step (env, .add e1 e2) (env', .add e1' e2)
   | add_right :
-    Reduce (env, e2) (env', e2') ->
-    Reduce (env, .add (.num n1) e2) (env', .add (.num n1) e2')
-  | add_val : Reduce (env, .add (.num n1) (.num n2)) (env, .num (n1 + n2))
+    Step (env, e2) (env', e2') ->
+    Step (env, .add (.num n1) e2) (env', .add (.num n1) e2')
+  | add_val :
+    Step (env, .add (.num n1) (.num n2)) (env, .num (n1 + n2))
   | mul_left :
-    Reduce (env, e1) (env', e1') ->
-    Reduce (env, .mul e1 e2) (env', .mul e1' e2)
+    Step (env, e1) (env', e1') ->
+    Step (env, .mul e1 e2) (env', .mul e1' e2)
   | mul_right :
-    Reduce (env, e2) (env', e2') ->
-    Reduce (env, .mul (.num n1) e2) (env', .mul (.num n1) e2')
-  | mul_val : Reduce (env, .mul (.num n1) (.num n2)) (env, .num (n1 * n2))
-  | val_reduce :
-    Reduce (env, e1) (env', e1') ->
-    Reduce (env, .val x e1 e2) (env', .val x e1' e2)
-  | val_val : Reduce (env, .val x (.num n) e2) (Env.update env x n, e2)
-  | id : env x = some n -> Reduce (env, .id x) (env, .num n)
+    Step (env, e2) (env', e2') ->
+    Step (env, .mul (.num n1) e2) (env', .mul (.num n1) e2')
+  | mul_val :
+    Step (env, .mul (.num n1) (.num n2)) (env, .num (n1 * n2))
+  | val_step :
+    Step (env, e1) (env', e1') ->
+    Step (env, .val x e1 e2) (env', .val x e1' e2)
+  | val_bind :
+    Step (env, .val x (.num n) e2) (env.insert x n, e2)
+  | id (h : x ∈ env) :
+    Step (env, .id x) (env, .num (env.get x h))
 
 -- multi-step evaluation relations (reflexive-transitive closure)
-inductive ReduceStar : Env × Expr -> Env × Expr -> Prop where
-  | refl : ReduceStar c c
-  | step : Reduce c c' -> ReduceStar c' c'' -> ReduceStar c c''
-
--- k-step evaluation relations
-inductive ReduceK : Nat -> Env × Expr -> Env × Expr -> Prop where
-  | refl : ReduceK 0 c c
-  | step : Reduce c c' -> ReduceK k c' c'' -> ReduceK (k + 1) c c''
-
--- ReduceK implies ReduceStar
-theorem ReduceK_to_ReduceStar (h : ReduceK k c c') : ReduceStar c c' := by
-  induction h with
-  | refl => exact ReduceStar.refl
-  | step hstep _ ih => exact ReduceStar.step hstep ih
+inductive MultiStep : Env × Expr -> Env × Expr -> Prop where
+  | refl : MultiStep c c
+  | step : Step c c' -> MultiStep c' c'' -> MultiStep c c''
 
 end VAE
