Verified/IMP/BigStep/Properties.lean
@@ -4,7 +4,6 @@ import Verified.IMP.BigStep
 namespace IMP
 
 -- Equivalence of Statements
-
 theorem while_unfold :
     Exec env (.while e s) env' <-> Exec env (.ite e (.seq s (.while e s)) .skip) env'
   := by
@@ -24,36 +23,40 @@ theorem while_unfold :
       cases hs with
       | skip => exact Exec.while_false he
 
--- Determinism of BigStep IMP
-
+-- Determinism of Expression Evaluation
 theorem Eval.deterministic (h1 : Eval env e v1) (h2 : Eval env e v2) :
-    v1 = v2 := by
+    v1 = v2
+  := by
   induction h1 generalizing v2 with
   | num => cases h2; rfl
   | bool => cases h2; rfl
-  | var h1 => cases h2 with
-    | var h2 => rw [h1] at h2; injection h2
+  | var _ => cases h2; rfl
   | add he1 he2 ih1 ih2 =>
     cases h2 with
     | add he1' he2' =>
-      have := ih1 he1'; injection this with this
-      have := ih2 he2'; injection this with this
-      subst_vars; rfl
+      have h1 := ih1 he1'
+      have h2 := ih2 he2'
+      simp only [Value.num.injEq] at h1 h2
+      subst h1; subst h2; rfl
   | mul he1 he2 ih1 ih2 =>
     cases h2 with
-      | mul he1' he2' =>
-        have := ih1 he1'; injection this with this
-        have := ih2 he2'; injection this with this
-        subst_vars; rfl
+    | mul he1' he2' =>
+      have h1 := ih1 he1'
+      have h2 := ih2 he2'
+      simp only [Value.num.injEq] at h1 h2
+      subst h1; subst h2; rfl
   | lt he1 he2 ih1 ih2 =>
     cases h2 with
     | lt he1' he2' =>
-      have := ih1 he1'; injection this with this
-      have := ih2 he2'; injection this with this
-      subst_vars; rfl
+      have h1 := ih1 he1'
+      have h2 := ih2 he2'
+      simp only [Value.num.injEq] at h1 h2
+      subst h1; subst h2; rfl
 
+-- Determinism of Statement Execution
 theorem Exec.deterministic (h1 : Exec env s env') (h2 : Exec env s env'') :
-    env' = env'' := by
+    env' = env''
+  := by
   induction h1 generalizing env'' with
   | skip => cases h2; rfl
   | assign heval =>
@@ -68,29 +71,27 @@ theorem Exec.deterministic (h1 : Exec env s env') (h2 : Exec env s env'') :
       exact ih2 hs2'
   | ite_true heval hs ih =>
     cases h2 with
-    | ite_true heval' hs' => exact ih hs'
-    | ite_false heval' hs' =>
+    | ite_true _ hs' => exact ih hs'
+    | ite_false heval' _ =>
       have := Eval.deterministic heval heval'
       cases this
   | ite_false heval hs ih =>
     cases h2 with
-    | ite_true heval' hs' =>
+    | ite_true heval' _ =>
       have := Eval.deterministic heval heval'
       cases this
-    | ite_false heval' hs' => exact ih hs'
+    | ite_false _ hs' => exact ih hs'
   | while_true heval hs hw ih_s ih_w =>
     cases h2 with
     | while_true heval' hs' hw' =>
       have := ih_s hs'; subst this
       exact ih_w hw'
     | while_false heval' =>
-      have := Eval.deterministic heval heval'
-      cases this
+      have := Eval.deterministic heval heval'; cases this
   | while_false heval =>
     cases h2 with
-    | while_true heval' hs' hw' =>
-      have := Eval.deterministic heval heval'
-      cases this
+    | while_true heval' _ _ =>
+      have := Eval.deterministic heval heval'; cases this
     | while_false => rfl
 
 end IMP
